Restore interop for gcm_encrypt, no admit_smt_queries left (EverCrypt.AEAD still failing)

vale/code/arch/x64/interop/Vale.Wrapper.X64.GCMencryptOpt.fst
@@ -138,7 +138,12 @@ val gcm128_encrypt_opt':
       (let db = get_downview hkeys_b in
        length_aux5 hkeys_b;
        let ub = UV.mk_buffer db Vale.Interop.Views.up_view128 in
-       hkeys_reqs_pub (UV.as_seq h0 ub) (reverse_bytes_quad32 (aes_encrypt_LE AES_128 (Ghost.reveal key) (Mkfour 0 0 0 0))))
+       hkeys_reqs_pub (UV.as_seq h0 ub) (reverse_bytes_quad32 (aes_encrypt_LE AES_128 (Ghost.reveal key) (Mkfour 0 0 0 0)))) /\
+
+      (length_div iv_b;
+       (reverse_bytes_quad32 (low_buffer_read TUInt8 TUInt128 h0 iv_b 0) ==
+         compute_iv_BE (aes_encrypt_LE AES_128 (Ghost.reveal key) (Mkfour 0 0 0 0)) (Ghost.reveal iv))
+      )
     )
     (ensures fun h0 _ h1 ->
       B.modifies (B.loc_union (B.loc_buffer tag_b)
@@ -164,10 +169,6 @@ val gcm128_encrypt_opt':
        let out128_d = get_downview out128_b in
        length_aux3 out128_b (UInt64.v len128_num);
        let out128_u = UV.mk_buffer out128_d Vale.Interop.Views.up_view128 in
-       length_aux4 iv_b;
-       length_div iv_b;
-       let iv_LE = low_buffer_read TUInt8 TUInt128 h0 iv_b 0 in
-       let iv_BE = reverse_bytes_quad32 iv_LE in
        let plain_in =
            Seq.append (Seq.append (UV.as_seq h0 in128x6_u) (UV.as_seq h0 in128_u))
                       (UV.as_seq h0 inout_u)
@@ -187,7 +188,7 @@ val gcm128_encrypt_opt':
       (Seq.length plain_bytes) < pow2_32 /\
       (Seq.length auth_bytes) < pow2_32 /\
       is_aes_key AES_128 (seq_nat32_to_seq_nat8_LE (Ghost.reveal key)) /\
-      (let cipher, tag = gcm_encrypt_LE AES_128 (seq_nat32_to_seq_nat8_LE (Ghost.reveal key)) (be_quad32_to_bytes iv_BE) plain_bytes auth_bytes in
+      (let cipher, tag = gcm_encrypt_LE AES_128 (seq_nat32_to_seq_nat8_LE (Ghost.reveal key)) (Ghost.reveal iv) plain_bytes auth_bytes in
       cipher == cipher_bytes /\
       (length_div tag_b;
       le_quad32_to_bytes (low_buffer_read TUInt8 TUInt128 h1 tag_b 0) == tag
@@ -350,7 +351,10 @@ val gcm128_encrypt_opt_alloca:
          (seq_nat8_to_seq_uint8 (le_seq_quad32_to_bytes (key_to_round_keys_LE AES_128 (Ghost.reveal key))))) /\
 
       hkeys_reqs_pub (le_bytes_to_seq_quad32 (seq_uint8_to_seq_nat8 (B.as_seq h0 hkeys_b)))
-        (reverse_bytes_quad32 (aes_encrypt_LE AES_128 (Ghost.reveal key) (Mkfour 0 0 0 0)))
+        (reverse_bytes_quad32 (aes_encrypt_LE AES_128 (Ghost.reveal key) (Mkfour 0 0 0 0))) /\
+
+      (be_bytes_to_quad32 (seq_uint8_to_seq_nat8 (B.as_seq h0 iv_b))) ==
+         compute_iv_BE (aes_encrypt_LE AES_128 (Ghost.reveal key) (Mkfour 0 0 0 0)) (Ghost.reveal iv)
     )
     (ensures fun h0 _ h1 ->
       B.modifies (B.loc_union (B.loc_buffer tag_b)
@@ -369,9 +373,6 @@ val gcm128_encrypt_opt_alloca:
        let out_d = get_downview out_b in
        length_aux3 out_b (UInt64.v plain_len / 16);
        let out_u = UV.mk_buffer out_d Vale.Interop.Views.up_view128 in
-       length_aux4 iv_b;
-       DV.length_eq (get_downview iv_b);
-       let iv = seq_uint8_to_seq_nat8 (B.as_seq h0 iv_b) in
        let plain_in = Seq.append (UV.as_seq h0 plain_u) (UV.as_seq h0 inout_u) in
        let plain_bytes = wrap_slice (le_seq_quad32_to_bytes plain_in) (UInt64.v plain_len) in
        let cipher_out = Seq.append (UV.as_seq h1 out_u) (UV.as_seq h1 inout_u) in
@@ -386,7 +387,7 @@ val gcm128_encrypt_opt_alloca:
       let auth_bytes = wrap_slice (le_seq_quad32_to_bytes auth_in) (UInt64.v auth_len) in
       Seq.length plain_bytes < pow2_32 /\
       Seq.length auth_bytes < pow2_32 /\
-      (let cipher, tag = gcm_encrypt_LE AES_128 (seq_nat32_to_seq_nat8_LE (Ghost.reveal key)) iv plain_bytes auth_bytes in
+      (let cipher, tag = gcm_encrypt_LE AES_128 (seq_nat32_to_seq_nat8_LE (Ghost.reveal key)) (Ghost.reveal iv) plain_bytes auth_bytes in
       Seq.equal cipher cipher_bytes /\
       Seq.equal (seq_uint8_to_seq_nat8 (B.as_seq h1 tag_b)) tag
       )
@@ -913,9 +914,6 @@ let gcm128_encrypt_opt_stdcall key iv plain_b plain_len auth_b auth_len iv_b out
        let out_d = get_downview out_b' in
        length_aux3 out_b' (UInt64.v plain_len / 16);
        let out_u = UV.mk_buffer out_d Vale.Interop.Views.up_view128 in
-       length_aux4 iv_b;
-       DV.length_eq (get_downview iv_b);
-       let iv = seq_uint8_to_seq_nat8 (B.as_seq h1 iv_b) in
        let plain_in = Seq.append (UV.as_seq h1 plain_u) (UV.as_seq h1 inout_u) in
        let plain_bytes = wrap_slice (le_seq_quad32_to_bytes plain_in) (UInt64.v plain_len) in
        let cipher_out = Seq.append (UV.as_seq h_post out_u) (UV.as_seq h_post inout_u) in
@@ -930,7 +928,7 @@ let gcm128_encrypt_opt_stdcall key iv plain_b plain_len auth_b auth_len iv_b out
        let auth_bytes = wrap_slice (le_seq_quad32_to_bytes auth_in) (UInt64.v auth_len) in
        (Seq.length plain_bytes) < pow2_32 /\
        (Seq.length auth_bytes) < pow2_32 /\
-       (let cipher, tag = gcm_encrypt_LE AES_128 (seq_nat32_to_seq_nat8_LE (Ghost.reveal key)) iv plain_bytes auth_bytes in
+       (let cipher, tag = gcm_encrypt_LE AES_128 (seq_nat32_to_seq_nat8_LE (Ghost.reveal key)) (Ghost.reveal iv) plain_bytes auth_bytes in
        Seq.equal cipher cipher_bytes /\
        Seq.equal (seq_uint8_to_seq_nat8 (B.as_seq h_post tag_b)) tag
   ));
@@ -964,10 +962,9 @@ let gcm128_encrypt_opt_stdcall key iv plain_b plain_len auth_b auth_len iv_b out
   lemma_slice_uv_extra out_b out_b' inout_b h2;
 
   assert (
-    let iv = seq_uint8_to_seq_nat8 (B.as_seq h1 iv_b) in
     let plain = seq_uint8_to_seq_nat8 (B.as_seq h1 plain_b) in
     let auth = seq_uint8_to_seq_nat8 (B.as_seq h1 auth_b) in
-    let cipher, tag = gcm_encrypt_LE AES_128 (seq_nat32_to_seq_nat8_LE (Ghost.reveal key)) iv plain auth in
+    let cipher, tag = gcm_encrypt_LE AES_128 (seq_nat32_to_seq_nat8_LE (Ghost.reveal key)) (Ghost.reveal iv) plain auth in
     Seq.equal (seq_uint8_to_seq_nat8 (B.as_seq h2 out_b)) cipher /\
     Seq.equal (seq_uint8_to_seq_nat8 (B.as_seq h2 tag_b)) tag);
 
