Makefile
@@ -481,10 +481,10 @@ obj/Vale.Wrapper.X64.GCMdecryptOpt.fst.checked: \
   FSTAR_FLAGS=$(VALE_FSTAR_FLAGS)
 
 obj/Vale.Wrapper.X64.GCMencryptOpt.fst.checked: \
-  FSTAR_FLAGS=$(VALE_FSTAR_FLAGS) --admit_smt_queries true
+  FSTAR_FLAGS=$(VALE_FSTAR_FLAGS)
 
 obj/Vale.Wrapper.X64.GCMencryptOpt256.fst.checked: \
-  FSTAR_FLAGS=$(VALE_FSTAR_FLAGS) --admit_smt_queries true
+  FSTAR_FLAGS=$(VALE_FSTAR_FLAGS)
 
 obj/Vale.Wrapper.X64.GCMdecryptOpt256.fst.checked: \
   FSTAR_FLAGS=$(VALE_FSTAR_FLAGS)
